closed denote/extract var

src/theories/Reflection/FM.v
@@ -36,6 +36,50 @@ Fixpoint dec_vars (t: term) : term :=
   | _ => t
   end.
 
+Fixpoint reindex_vars (t: term) : term :=
+  match t with
+  | tCast from kind to => 
+    tCast (reindex_vars from) kind (reindex_vars to)
+  | tProd na ty body => 
+    let bod' := reindex_vars body in 
+    let bod'' := 
+      match na.(binder_name) with 
+      | nAnon => dec_vars bod'
+      | _ => bod'
+      end in
+    tProd na (reindex_vars ty) bod''
+  | tLambda na ty body => 
+    tLambda na (reindex_vars ty) (reindex_vars body)
+  | tLetIn na def def_ty body =>
+    tLetIn na (reindex_vars def) (reindex_vars def_ty) (reindex_vars body)
+  | tApp f args => 
+    tApp (reindex_vars f) (map reindex_vars args)
+  | tCase ind_nbparams_relevance type_info discr branches =>
+    tCase ind_nbparams_relevance (reindex_vars type_info) (reindex_vars discr) (List.map (fun '(n, t) => (n, reindex_vars t)) branches)
+  | tProj proj t0 => tProj proj (reindex_vars t0)
+  | _ => t
+  end.
+
+Section Lenses.
+  Variable (s: signature).
+  Variable (m: model s).
+  Equations mk_var (c: ctx s) (v: valu s m c) (n: nat) : option ({ty & s.(mod_sorts) m ty * var s c ty})%type by struct c := 
+    mk_var SLNil _ _ := None;
+    (* ugh auto-generated names... *)
+    mk_var (Snoc _ srt) (VSnoc _ _ _ x) 0 := Some (v; (x, VHere _ _ _));
+    mk_var (Snoc c' ty) (VSnoc _ _ v _) (S n) := 
+      (* 
+        c' is v1, ty is v0, v is v, n is n
+      *)
+      match mk_var v1 v n with 
+      | Some (ty; (r, v')) => Some (ty; (r, VThere _ _ _ _ v'))
+      | None => None
+      end.
+
+  (* Parameter dummy_valu : forall (c: ctx s), valu s m c. *)
+
+End Lenses.
+
 Section ExtractFM.
   Variable (s: signature).
   Variable (m: model s).
@@ -45,33 +89,29 @@ Section ExtractFM.
 
   Variable (sort_eq_dec: EquivDec.EqDec (sig_sorts s) eq).
 
-  Equations mk_var (c: ctx s) (n: nat) : option ({srt & var s c srt}) by struct n := 
-    mk_var (Snoc _ c' srt) 0 := Some (existT _ srt (VHere _ _ srt));
-    mk_var (Snoc _ c' srt) (S n') := 
-      let nxt := mk_var c' n' in 
-      match nxt with 
-      | Some v =>
-        let (ty', v') := v in 
-        Some (existT _ ty' (VThere _ _ _ _ v'))
+  Equations extract_var (c: ctx s) (n: nat) : option ({srt & var s c srt}) by struct c :=
+    extract_var (Snoc _ _ ty) 0 := Some (ty; VHere _ _ ty);
+    extract_var (Snoc _ c _) (S n) :=
+      match extract_var c n with
+      | Some (ty; v') => Some (ty; VThere _ _ _ _ v')
       | None => None
       end;
-    mk_var SLNil _ := None.
+    extract_var SLNil _ := None.
 
-  Fixpoint extract_t2tm' (c: ctx s) (acc: nat) (t: term) : option ({srt & tm s c srt}) :=  
+  Fixpoint extract_t2tm' (c: ctx s) (t: term) : option ({srt & tm s c srt}) :=  
     match t with 
     | tRel n => 
-      match mk_var c (n - acc) with 
-      | Some (existT srt v) => 
-        Some (existT _ srt (TVar v))
+      match extract_var c n with 
+      | Some (ty; v) => Some (ty; TVar v)
       | None => None
       end
-    | tApp f es => extract_t2tm c t (map (extract_t2tm' c acc) es)
+    | tApp f es => extract_t2tm c t (map (extract_t2tm' c) es)
     | _ => extract_t2tm c t []
     end.
 
   Obligation Tactic := intros.
-  Equations extract_t2fm (c: ctx s) (anon_acc: nat) (t: term) : option (fm _ c) by struct t := 
-    extract_t2fm c acc t := 
+  Equations extract_t2fm (c: ctx s) (t: term) : option (fm _ c) by struct t := 
+    extract_t2fm c t := 
       if eq_term t c_True then Some FTrue else 
       if eq_term t c_False then Some FFalse else
       match t with
@@ -79,7 +119,7 @@ Section ExtractFM.
         if eq_term f c_eq then 
           match es with 
           | _ :: tl :: tr :: _ => 
-            match extract_t2tm' c acc tl, extract_t2tm' c acc tr with 
+            match extract_t2tm' c tl, extract_t2tm' c tr with 
             | Some l, Some r => 
               let (sl, el) := l in 
               let (sr, er) := r in 
@@ -95,7 +135,7 @@ Section ExtractFM.
         else if eq_term f c_or then 
           match es with 
           | tl :: tr :: _ => 
-            match extract_t2fm c acc tl, extract_t2fm c acc tr with 
+            match extract_t2fm c tl, extract_t2fm c tr with 
             | Some l, Some r => Some (@FOr _ c l r)
             | _, _ => None
             end
@@ -104,7 +144,7 @@ Section ExtractFM.
         else if eq_term f c_and then 
           match es with 
           | tl :: tr :: _ => 
-            match extract_t2fm c acc tl, extract_t2fm c acc tr with 
+            match extract_t2fm c tl, extract_t2fm c tr with 
             | Some l, Some r => Some (@FAnd _ c l r)
             | _, _ => None
             end
@@ -113,7 +153,7 @@ Section ExtractFM.
         else if eq_term f c_not then 
           match es with 
           | x :: _ => 
-            match extract_t2fm c acc x with 
+            match extract_t2fm c x with 
             | Some x' => Some (FNeg _ x')
             | None => None
             end
@@ -124,7 +164,7 @@ Section ExtractFM.
       | tProd ba_name pre pst => 
         match ba_name.(binder_name) with 
         | nAnon => 
-          match extract_t2fm c acc pre, extract_t2fm c (S acc) pst with 
+          match extract_t2fm c pre, extract_t2fm c pst with 
           | Some el, Some er => Some (FImpl el er)
           | _, _ => None
           end
@@ -133,7 +173,7 @@ Section ExtractFM.
           match srt with 
           | Some srt => 
             let c' := Snoc _ c srt in
-            let inner := extract_t2fm c' acc pst in 
+            let inner := extract_t2fm c' pst in 
             match inner with 
             | Some fm => Some (FForall _ fm)
             | None => None
@@ -145,26 +185,27 @@ Section ExtractFM.
       | _ => None
       end.
 
+  Definition extract_fm t := extract_t2fm (SLNil _) (reindex_vars t).
+
   (* Some light tests *)
-  (* Variable (c: ctx s).
+  Variable (c: ctx s).
 
   MetaCoq Quote Definition test_1 := (False -> True).
   MetaCoq Quote Definition test_2 := (True = False -> False).
   MetaCoq Quote Definition test_3 := (~ ~ False).
   MetaCoq Quote Definition test_4 := (False /\ True).
-  MetaCoq Quote Definition test_5 := (forall (x: unit), True).
+  MetaCoq Quote Definition test_5 := (forall (x: unit), True -> True).
   MetaCoq Quote Definition test_6 := (forall (x: unit), True \/ False \/ ~ True).
 
-  Eval vm_compute in extract_t2fm c 0 test_1.
-  Eval vm_compute in extract_t2fm c 0 test_2. 
-  Eval vm_compute in extract_t2fm c 0 test_3.
-  Eval vm_compute in extract_t2fm c 0 test_4.
-  Eval vm_compute in extract_t2fm c 0 test_5.
-  Eval vm_compute in extract_t2fm c 0 test_6. *)
+  (* Eval vm_compute in extract_fm test_1.
+  Eval vm_compute in extract_fm test_2.
+  Eval vm_compute in extract_fm test_3.
+  Eval vm_compute in extract_fm test_4.
+  Eval vm_compute in extract_fm test_5.
+  Eval vm_compute in extract_fm test_6. *)
+  
 End ExtractFM.
     
-
-
 
 Section DenoteFM.
 
@@ -174,29 +215,32 @@ Section DenoteFM.
   Variable (sorts_eq_dec: EquivDec.EqDec (s.(sig_sorts)) eq).
 
   Notation res_ty := (option ({ty & s.(mod_sorts) m ty})).
-  (* Notation env_ty := ({c & valu s m c}). *)
   Notation env_ty c := (valu s m c).
 
   Variable (denote_tm : term -> list res_ty -> res_ty).
   Variable (reify_srt : term -> option (s.(sig_sorts))).
 
   Fixpoint denote_var {c} (env: env_ty c) (n: nat) : res_ty :=
-    match env, n with 
-    | VSnoc _ _ _ x, 0 => Some (existT _ _ x)
+    match env, n with
+    | VSnoc _ _ _ x, 0 => Some (_; x)
     | VSnoc _ _ env' _, S n' => denote_var env' n'
     | VEmp, _ => None
     end.
 
-  Fixpoint denote_tm' {c} (env: env_ty c) (acc: nat) (t: term) : res_ty :=  
+  Fixpoint denote_tm' {c} (env: env_ty c) (t: term) : res_ty :=  
     match t with 
-    | tRel n => denote_var env (n - acc)
-    | tApp f es => denote_tm t (map (denote_tm' env acc) es)
+    | tRel n => 
+      match denote_var env n with 
+      | Some (ty; r) => Some (ty; r)
+      | None => None
+      end
+    | tApp f es => denote_tm t (map (denote_tm' env) es)
     | _ => denote_tm t []
     end.
 
   Obligation Tactic := intros.
-  Equations denote_t2fm {c} (env: env_ty c) (anon_acc: nat) (t: term) : Prop by struct t := 
-    denote_t2fm env acc t := 
+  Equations denote_t2fm {c} (env: env_ty c) (t: term) : Prop by struct t := 
+    denote_t2fm env t := 
       if eq_term t c_True then True else 
       if eq_term t c_False then False else
       match t with
@@ -204,7 +248,7 @@ Section DenoteFM.
         if eq_term f c_eq then 
           match es with 
           | _ :: tl :: tr :: _ => 
-            match denote_tm' env acc tl, denote_tm' env acc tr with 
+            match denote_tm' env tl, denote_tm' env tr with 
             | Some l, Some r => 
               let (tl, el) := l in 
               let (tr, er) := r in 
@@ -219,46 +263,41 @@ Section DenoteFM.
           end
         else if eq_term f c_or then 
           match es with 
-          | tl :: tr :: _ => denote_t2fm env acc tl \/ denote_t2fm env acc tr
+          | tl :: tr :: _ => denote_t2fm env tl \/ denote_t2fm env tr
           | _ => False
           end
         else if eq_term f c_and then 
           match es with 
-          | tl :: tr :: _ => denote_t2fm env acc tl /\ denote_t2fm env acc tr
+          | tl :: tr :: _ => denote_t2fm env tl /\ denote_t2fm env tr
           | _ => False
           end
         else if eq_term f c_not then 
           match es with 
-          | x :: _ => ~ denote_t2fm env acc x
+          | x :: _ => ~ denote_t2fm env x
           | _ => False
           end
         else
           False
       | tProd ba_name pre pst => 
         match ba_name.(binder_name) with 
-        | nAnon => denote_t2fm env acc pre -> denote_t2fm env (S acc) pst
+        | nAnon => denote_t2fm env pre -> denote_t2fm env pst
         | nNamed _ =>
           match reify_srt pre with
           | Some ty' => 
             forall x: (s.(mod_sorts) m ty'), 
-              denote_t2fm (VSnoc _ _ ty' c env x) acc pst 
+              denote_t2fm (VSnoc _ _ ty' c env x) pst 
           | None => False
           end
         end
       | _ => False
       end.
 
-  (* MetaCoq Quote Definition test_1 := (False -> True).
-  MetaCoq Quote Definition test_2 := (True = False -> False).
-  MetaCoq Quote Definition test_3 := (~ ~ False).
-  MetaCoq Quote Definition test_4 := (False /\ True).
-  MetaCoq Quote Definition test_5 := (forall (x: unit), x = tt).
-  MetaCoq Quote Definition test_6 := (forall (x: unit), True \/ False \/ ~ True). *)
+  Definition denote_fm t := denote_t2fm (VEmp _ _) (reindex_vars t).
 
-  (* Eval vm_compute in denote_t2fm (VEmp _ _)  0 test_1.
-  Eval vm_compute in denote_t2fm (VEmp _ _)  0 test_2. 
-  Eval vm_compute in denote_t2fm (VEmp _ _)  0 test_3.
-  Eval vm_compute in denote_t2fm (VEmp _ _)  0 test_4.
-  Eval vm_compute in denote_t2fm (VEmp _ _)  0 test_5.
-  Eval vm_compute in denote_t2fm (VEmp _ _)  0 test_6. *)
+  (* Eval vm_compute in denote_fm test_1.
+  Eval vm_compute in denote_fm test_2.
+  Eval vm_compute in denote_fm test_3.
+  Eval vm_compute in denote_fm test_4.
+  Eval vm_compute in denote_fm test_5.
+  Eval vm_compute in denote_fm test_6. *)
 End DenoteFM.
